examples/Driver.v
@@ -1,0 +1,4 @@
+Require Isa Add.
+
+Definition example1 := Isa.t. 
+Definition example2 := (Compiler.copt _ _  (Add.test 3)).
