examples/Extraction.v
@@ -1,0 +1,62 @@
+Require Driver. 
+
+Set Extraction AccessOpaque.
+
+Cd "tmp".
+
+Extraction Blacklist String List.
+
+Extract Inductive bool => bool [ true false ].
+Extract Inductive option => option [ Some None ].
+Extract Inductive unit => unit [ "()" ].
+Extract Inductive list => list [ "[]" "( :: )" ].
+Extract Inductive prod => "( * )" [ "" ].
+
+(** NB: The "" above is a hack, but produce nicer code than "(,)" *)
+
+(** Mapping sumbool to bool and sumor to option is not always nicer,
+    but it helps when realizing stuff like [lt_eq_lt_dec] *)
+
+Extract Inductive sumbool => bool [ true false ].
+Extract Inductive sumor => option [ Some None ].
+
+(** Restore lazyness of andb, orb.
+    NB: without these Extract Constant, andb/orb would be inlined
+    by extraction in order to have lazyness, producing inelegant
+    (if ... then ... else false) and (if ... then true else ...).
+*)
+
+Extract Inlined Constant andb => "(&&)".
+Extract Inlined Constant orb => "(||)".
+
+Extract Constant Common.admit => "Obj.magic ()".
+
+Extract Inductive nat => int [ "0" "Pervasives.succ" ]
+ "(fun fO fS n -> if n=0 then fO () else fS (n-1))".
+
+(** Efficient (but uncertified) versions for usual [nat] functions *)
+
+Extract Constant plus => "(+)".
+Extract Constant pred => "fun n -> max 0 (n-1)".
+Extract Constant minus => "fun n m -> max 0 (n-m)".
+Extract Constant mult => "( * )".
+Extract Inlined Constant max => max.
+Extract Inlined Constant min => min.
+(*Extract Inlined Constant nat_beq => "(=)".*)
+Extract Inlined Constant EqNat.beq_nat => "(=)".
+Extract Inlined Constant EqNat.eq_nat_decide => "(=)".
+
+Extract Inlined Constant Peano_dec.eq_nat_dec => "(=)".
+
+Extract Constant Compare_dec.nat_compare =>
+ "fun n m -> if n=m then Eq else if n<m then Lt else Gt".
+Extract Inlined Constant Compare_dec.leb => "(<=)".
+Extract Inlined Constant Compare_dec.le_lt_dec => "(<=)".
+Extract Constant Compare_dec.lt_eq_lt_dec =>
+ "fun n m -> if n>m then None else Some (n<m)".
+
+Extract Constant Even.even_odd_dec => "fun n -> n mod 2 = 0".
+Extract Constant Div2.div2 => "fun n -> n/2".
+
+Recursive Extraction Library Driver. 
+
